code/sha2-vec/Hacl.Impl.SHA2.Core.fsti
@@ -1,52 +1,134 @@
 module Hacl.Impl.SHA2.Core
-open FStar.Mul
-module ST = FStar.HyperStack.ST
+
 open FStar.HyperStack
 open FStar.HyperStack.All
+open FStar.Mul
+
 open Lib.IntTypes
-open Lib.Sequence
 open Lib.Buffer
-open Lib.IntVector
 open Lib.MultiBuffer
+
 open Spec.Hash.Definitions
 open Hacl.Hash.Definitions
-module Spec = Hacl.Spec.SHA2
+open Hacl.Spec.SHA2.Vec
 
-val sha256: hash:lbuffer uint8 32ul -> len:size_t -> b:lbuffer uint8 len ->
-    Stack unit
-    (requires (fun h0 -> live h0 b /\ live h0 hash /\ disjoint hash b))
-    (ensures (fun h0 _ h1 -> modifies (loc hash) h0 h1 /\
-                           as_seq h1 hash == Spec.hash #SHA2_256 (v len) (as_seq h0 b)))
+module SpecVec = Hacl.Spec.SHA2.Vec
 
+#set-options "--z3rlimit 50 --fuel 0 --ifuel 0"
 
-val sha256_4 (r0 r1 r2 r3: lbuffer uint8 32ul)
-             (len:size_t)
-             (b0 b1 b2 b3: lbuffer uint8 len) :
-    Stack unit
-    (requires (fun h0 -> live4 h0 b0 b1 b2 b3 /\
-                       live4 h0 r0 r1 r2 r3 /\
-                       internally_disjoint4 r0 r1 r2 r3))
-    (ensures (fun h0 _ h1 -> modifies (loc r0 |+| loc r1 |+| loc r2 |+| loc r3) h0 h1 /\
-                           as_seq h1 r0 == Spec.hash #SHA2_256 (v len) (as_seq h0 b0) /\
-                           as_seq h1 r1 == Spec.hash #SHA2_256 (v len) (as_seq h0 b1) /\
-                           as_seq h1 r2 == Spec.hash #SHA2_256 (v len) (as_seq h0 b2) /\
-                           as_seq h1 r3 == Spec.hash #SHA2_256 (v len) (as_seq h0 b3)))
+unfold
+let state_t (a:sha2_alg) (m:m_spec) =
+  lbuffer (element_t a m) 8ul
+
+inline_for_extraction noextract
+let init_vec_t (a:sha2_alg) (m:m_spec) = hash:state_t a m ->
+  Stack unit
+  (requires fun h -> live h hash)
+  (ensures  fun h0 _ h1 -> modifies1 hash h0 h1 /\
+    as_seq h1 hash == SpecVec.init a m)
+
+inline_for_extraction noextract
+val init: #a:sha2_alg -> #m:m_spec -> init_vec_t a m
 
 
+inline_for_extraction noextract
+let update_vec_t (a:sha2_alg) (m:m_spec) =
+    b:multibuf (lanes a m) (block_len a)
+  -> hash:state_t a m ->
+  Stack unit
+  (requires fun h -> live_multi h b /\ live h hash)
+  (ensures  fun h0 _ h1 -> modifies (loc hash) h0 h1 /\
+    as_seq h1 hash == SpecVec.update (as_seq_multi h0 b) (as_seq h0 hash))
 
-val sha256_8 (r0 r1 r2 r3 r4 r5 r6 r7 : lbuffer uint8 32ul)
-             (len:size_t)
-             (b0 b1 b2 b3 b4 b5 b6 b7 : lbuffer uint8 len) :
-    Stack unit
-    (requires (fun h0 -> live8 h0 b0 b1 b2 b3 b4 b5 b6 b7 /\ live8 h0 r0 r1 r2 r3 r4 r5 r6 r7 /\
-                       internally_disjoint8 r0 r1 r2 r3 r4 r5 r6 r7))
-    (ensures (fun h0 _ h1 -> modifies (loc r0 |+| loc r1 |+| loc r2 |+| loc r3 |+| loc r4 |+| loc r5 |+| loc r6 |+| loc r7) h0 h1 /\
-                           as_seq h1 r0 == Spec.hash #SHA2_256 (v len) (as_seq h0 b0) /\
-                           as_seq h1 r1 == Spec.hash #SHA2_256 (v len) (as_seq h0 b1) /\
-                           as_seq h1 r2 == Spec.hash #SHA2_256 (v len) (as_seq h0 b2) /\
-                           as_seq h1 r3 == Spec.hash #SHA2_256 (v len) (as_seq h0 b3) /\
-                           as_seq h1 r4 == Spec.hash #SHA2_256 (v len) (as_seq h0 b4) /\
-                           as_seq h1 r5 == Spec.hash #SHA2_256 (v len) (as_seq h0 b5) /\
-                           as_seq h1 r6 == Spec.hash #SHA2_256 (v len) (as_seq h0 b6) /\
-                           as_seq h1 r7 == Spec.hash #SHA2_256 (v len) (as_seq h0 b7)))
+inline_for_extraction noextract
+val update: #a:sha2_alg -> #m:m_spec -> update_vec_t a m
 
+
+inline_for_extraction noextract
+let update_last_vec_t (a:sha2_alg) (m:m_spec) =
+    upd:update_vec_t a m
+  -> totlen:len_t a
+  -> len:size_t{v len < block_length a}
+  -> b:multibuf (lanes a m) len
+  -> hash:state_t a m ->
+  Stack unit
+  (requires fun h -> live_multi h b /\ live h hash /\ disjoint_multi b hash)
+  (ensures  fun h0 _ h1 -> modifies (loc hash) h0 h1 /\
+    as_seq h1 hash == SpecVec.update_last totlen (v len) (as_seq_multi h0 b) (as_seq h0 hash))
+
+inline_for_extraction noextract
+val update_last: #a:sha2_alg -> #m:m_spec -> update_last_vec_t a m
+
+
+noextract
+let preserves_disjoint_multi #lanes #len #len' (b:multibuf lanes len) (r:multibuf lanes len') =
+    (forall a l (x:lbuffer a l). disjoint_multi b x ==> disjoint_multi r x)
+
+inline_for_extraction noextract
+let get_multiblock_t (a:sha2_alg) (m:m_spec) =
+    len:size_t
+  -> b:multibuf (lanes a m) len
+  -> i:size_t{v i < v len / block_length a} ->
+  Stack (multibuf (lanes a m) (block_len a))
+  (requires fun h -> live_multi h b)
+  (ensures  fun h0 r h1 -> h0 == h1 /\ live_multi h1 r /\ preserves_disjoint_multi b r /\
+    as_seq_multi h1 r == SpecVec.get_multiblock_spec (v len) (as_seq_multi h0 b) (v i))
+
+inline_for_extraction noextract
+val get_multiblock: #a:sha2_alg -> #m:m_spec -> get_multiblock_t a m
+
+
+inline_for_extraction noextract
+let get_multilast_t (a:sha2_alg) (m:m_spec) =
+    len:size_t
+  -> b:multibuf (lanes a m) len ->
+  Stack (multibuf (lanes a m) (len %. block_len a))
+  (requires fun h -> live_multi h b)
+  (ensures  fun h0 r h1 -> h0 == h1 /\ live_multi h1 r /\ preserves_disjoint_multi b r /\
+    as_seq_multi h1 r == SpecVec.get_multilast_spec #a #m (v len) (as_seq_multi h0 b))
+
+inline_for_extraction noextract
+val get_multilast: #a:sha2_alg -> #m:m_spec -> get_multilast_t a m
+
+
+inline_for_extraction noextract
+let update_nblocks_vec_t (a:sha2_alg) (m:m_spec) =
+    upd:update_vec_t a m
+  -> len:size_t
+  -> b:multibuf (lanes a m) len
+  -> st:state_t a m ->
+  Stack unit
+  (requires fun h0 -> live_multi h0 b /\ live h0 st /\ disjoint_multi b st)
+  (ensures  fun h0 _ h1 -> modifies (loc st) h0 h1 /\
+    as_seq h1 st == SpecVec.update_nblocks #a #m (v len) (as_seq_multi h0 b) (as_seq h0 st))
+
+inline_for_extraction noextract
+val update_nblocks: #a:sha2_alg -> #m:m_spec -> update_nblocks_vec_t a m
+
+
+inline_for_extraction noextract
+let finish_vec_t (a:sha2_alg) (m:m_spec) =
+    st:state_t a m
+  -> h:multibuf (lanes a m) (hash_len a) ->
+  Stack unit
+  (requires fun h0 -> live_multi h0 h /\ internally_disjoint h /\ live h0 st /\ disjoint_multi h st)
+  (ensures  fun h0 _ h1 -> modifies (loc_multi h |+| loc st) h0 h1 /\
+    as_seq_multi h1 h == SpecVec.finish #a #m (as_seq h0 st))
+
+inline_for_extraction noextract
+val finish: #a:sha2_alg -> #m:m_spec -> finish_vec_t a m
+
+
+inline_for_extraction noextract
+let hash_vec_t (a:sha2_alg) (m:m_spec) =
+    upd:update_vec_t a m
+  -> h:multibuf (lanes a m) (hash_len a)
+  -> len:size_t
+  -> b:multibuf (lanes a m) len ->
+  Stack unit
+  (requires fun h0 -> live_multi h0 b /\ live_multi h0 h /\ internally_disjoint h)
+  (ensures  fun h0 _ h1 -> modifies_multi h h0 h1 /\
+    as_seq_multi h1 h == SpecVec.hash #a #m (v len) (as_seq_multi h0 b))
+
+inline_for_extraction noextract
+val hash: #a:sha2_alg -> #m:m_spec -> hash_vec_t a m
